Fill View Change msg with full or empty Prepared Certificates.
In the View Change message we need to put for each Sequence ID
either a valid Prepared certificate with at least 2F+1 Prepares
or an empty Prepared certificate indicating we have no reason to
believe anything was committed for the given Sequence ID.

messages.dfy
@@ -25,6 +25,9 @@ module Messages {
                           && v1 != v2
                             :: v1.sender != v2.sender) // unique senders
     }
+    predicate empty() {
+      && |votes| == 0
+    }
   }
 
   // Define your Message datatype here.
